\documentclass{scrartcl}

\usepackage[english]{babel}
\usepackage[utf8]{inputenc}

\usepackage{amsmath}
\usepackage{amssymb}

\newcommand{\exd}{\mathbf{d}}
\newcommand{\Div}{\text{Div}}
\newcommand{\Rot}{\text{Rot}}
\newcommand{\vecflat}[1]{\vec{#1}^{\,\flat}}
\renewcommand{\i}{\mathbf{i}}
\renewcommand{\L}{\mathbf{\mathcal{L}}}


\begin{document}
\hoffset = -30pt

  \section{Arbitrary s.p.d. metric}
    \subsection{Assumptions}
      \begin{itemize}
        \item \( Ind(M) = 0 \)
        \item \( g =
      \begin{bmatrix}
        g_{11} & g_{12} \\
        g_{12} & g_{22}
      \end{bmatrix}  = g_{11}\left( dx^{1} \right)^{2} + 2g_{12}dx^{1}dx^{2} + g_{22}\left( dx^{2} \right)^{2}
        (\textbf{s.p.d.}) \)
      \end{itemize}

    \subsection{General proberties}
      \( \alpha \in \Omega^{p}(M) \),  \( \beta \in \Omega^{q}(M) \),  \( \gamma \in \Omega^{r}(M) \),
      \( \vec{v} \in \mathcal{V}(M) \)
      \subsubsection{Wedge product \( \wedge \)}
      \begin{itemize}
        \item \( \alpha\wedge\beta = (-1)^{pq}\beta\wedge\alpha \)
            (\textbf{anti-/commutativ})
        \item \textbf{associativ} (\( \alpha\wedge\beta\wedge\gamma \))
        \item \( \left( c_{1}\alpha + c_{2}\beta \right)\wedge\gamma
                  = c_{1}\alpha\wedge\gamma + c_{2}\beta\wedge\gamma\)
              (\textbf{bilinear})
      \end{itemize}

      \subsubsection{Exterior derivative \( \exd:\Omega^{p}(M)\rightarrow\Omega^{p+1}(M) \)}
        \( \alpha\in\Omega^{p}(M) \)
        \begin{itemize}
          \item \( \exd\circ\exd = 0 \) (\textbf{complex proberty})
          \item \( \exd\left( \alpha \wedge \beta \right) = \exd\alpha\wedge\beta + (-1)^{p}\alpha\wedge\exd\beta \)
                (\textbf{product rule, \( \wedge \)-antiderivation})
        \end{itemize}

      \subsubsection{Hodge star \( *:\Omega^{p}(M)\rightarrow\Omega^{2-p}(M) \)}
        \begin{itemize}
          \item \( \alpha \wedge *\beta = \beta \wedge *\alpha = \left\langle \alpha,\beta \right\rangle\mu \)
          \item \( *1 = \mu \) \quad(\( *\mu = 1 \))
          \item \( **\alpha = (-1)^{p}\alpha \)
          \item \( \left\langle \alpha, \beta \right\rangle =  \left\langle *\alpha, *\beta \right\rangle\)
        \end{itemize}

      \subsubsection{Contraction \( \i:\left(\mathcal{V}\times\Omega^{p}\right)(M)\rightarrow\Omega^{p-1}(M) \) (inner product)}
        \begin{itemize}
          \item \( \i_{\vec{v}}\alpha\left( \vec{t}_{1},\ldots\vec{t}_{p-1} \right) = \alpha\left(\vec{v}, \vec{t}_{1},\ldots\vec{t}_{p-1} \right) \)
          \item \( f\i_{\vec{v}}\alpha = \i_{f\vec{v}}\alpha 
                                       = \i_{\vec{v}}f\alpha \)
                (\textbf{bilinear})
          \item \( \i_{\vec{v}}\left( \alpha\wedge\beta \right) 
                    = \left( \i_{\vec{v}}\alpha \right)\wedge\beta + (-1)^{p}\alpha\wedge\left( \i_{\vec{v}}\beta \right)\)
                (\textbf{\( \wedge \)-antiderivation})
        \end{itemize}

      \subsubsection{Lie-derivative \( \L:\left(\mathcal{V}\times\Omega^{p}\right)(M)\rightarrow\Omega^{p}(M) \)}
        \begin{itemize}
          \item \(\L_{\vec{v}}\alpha = \i_{\vec{v}}\exd\alpha + \exd\i_{\vec{v}}\alpha\) 
          (\textbf{Cartans magic formular})
          \item  \( \L_{f\vec{v}}\alpha = f\L_{\vec{v}}\alpha + \exd f\wedge\i_{\vec{v}}\alpha\)
          \item \( \L_{\vec{v}}\left( \alpha\wedge\beta \right) = \L_{\vec{v}}\alpha\wedge\beta + \alpha\wedge\L_{\vec{v}}\beta\)
          \item \(\L_{\vec{v}}\exd\alpha = \exd\L_{\vec{v}}\alpha \)
          \item \(\L_{\vec{v}}\i_{\vec{v}}\alpha = \i_{\vec{v}}\L_{\vec{v}}\alpha \)\\
                \( \Rightarrow \alpha\in\Omega^{1}(M):\ \L_{\vec{v}} \left\langle \vecflat{v}, \alpha \right\rangle  
                                                          = \left\langle \vecflat{v}, \L_{\vec{v}}\alpha \right\rangle\)
          \item \( \L_{\vec{v}}\vec{w} = \left[ \vec{v} , \vec{w} \right] = \nabla_{\vec{v}}\vec{w} - \nabla_{\vec{w}}\vec{v}\)
          (\textbf{(Levi-Civita-)Conection \( \nabla \) is Torsion-free})
        \end{itemize}

    \subsection{Wedge product \( \wedge \)}
      \( f\in \Omega^{0}(M)\),
      \( \tilde{f}\in \Omega^{0}(M) \),
      \( \alpha:= a_{1}dx^{1} + a_{2}dx^{2} \in \Omega^{1}(M) \),
      \( \beta:= b_{1}dx^{1} + b_{2}dx^{2} \in \Omega^{1}(M) \),
      \( \omega:= w_{12}dx^{1}\wedge dx^{2} \in \Omega^{2}(M) \)
      \begin{itemize}
        \item \( f\tilde{f}= f\wedge\tilde{f} = \tilde{f}\wedge f \in \Omega^{0}(M) \)
        \item \( f\alpha := f\wedge\alpha = \alpha\wedge f =  fa_{1}dx^{1} + fa_{2}dx^{2} \in \Omega^{1}(M)\)
        \item \( \alpha\wedge\beta = - \beta\wedge\alpha = \left( a_{1}b_{2} - a_{2}b_{1} \right) dx^{1}\wedge dx^{2} \in \Omega^{2}(M) \)
        \item \( f\omega := f\wedge\omega = \omega\wedge f = fw_{12}dx^{1}\wedge dx^{2} \in \Omega^{2}(M) \)
      \end{itemize}
      
    \subsection{Exterior derivative \( \exd \)}
      \( f\in \Omega^{0}(M)\), 
      \( \alpha:= a_{1}dx^{1} + a_{2}dx^{2} \in \Omega^{1}(M) \)
      \begin{itemize}
        \item \( \exd f = \partial_{1}fdx^{1} + \partial_{2}fdx^{2} \)
        \item \( \left( \exd f \right)_{\mu} = \partial_{\mu}f \)  (\textbf{Ricci})
        \item \( \exd\alpha = \left( \partial_{1}a_{2} - \partial_{2}a_{1} \right) dx^{1}\wedge dx^{2}\)
        \item \( (\exd\alpha)_{12} = (-1)^{\mu-1}\partial_{\mu}a_{\bar{\mu}} \) (\textbf{Ricci})
      \end{itemize}

    \subsection{Hodge star \( * \)}
      \( f\in \Omega^{0}(M)\),
      \( \alpha:= a_{1}dx^{1} + a_{2}dx^{2} \in \Omega^{1}(M) \),
      \( \omega:= w_{12}dx^{1}\wedge dx^{2} \in \Omega^{2}(M) \)
      \begin{itemize}
        \item \( *f = f\mu = \sqrt{|g|}f dx^{1}\wedge dx^{2}\)
        \item \( *\alpha = \sqrt{|g|}\left( -\left( a_{1}g^{12} + a_{2}g^{22} \right)dx^{1} 
                                            +\left( a_{1}g^{11} + a_{2}g^{12} \right)dx^{2}\right) \)
        \item \( (*a)_{\mu} =  \left( -1 \right)^{\mu} \sqrt{|g|} g^{\nu\bar{\mu}}a_{\nu}
                          = \left( -1 \right)^{\mu} \sqrt{|g|} a^{\bar{\mu}}\)
                          (\textbf{Ricci})
        \item \( *\omega = \frac{w_{12}}{\sqrt{|g|}} \)
      \end{itemize}

    \subsection{Rising and lowering indices \( \sharp \) / \( \flat \)}
      \( \alpha:= a_{1}dx^{1} + a_{2}dx^{2} \in \Omega^{1}(M) \),
      \( \vec{v} := v^{1}\partial_{1} + v^{2}\partial_{2}\in\mathcal{V}(M) \)
      \begin{itemize}
        \item \( \alpha^{\sharp} = \left( g^{11}a_{1}+g^{12}a_{2} \right)\partial_{1} + \left( g^{12}a_{1}+g^{22}a_{2} \right)\partial_{2}\)
        \item \( a^{\mu} = g^{\mu\nu}a_{\nu}\) (\textbf{Ricci})
        \item \( \vecflat{v} = \left( g_{11}v^{1} + g_{12}v^{2} \right)dx^{1} + \left( g_{12}v^{1} + g_{22}v^{2} \right)dx^{2} \)
        \item \( v_{\mu} = g_{\mu\nu}v^{\nu} \) (\textbf{Ricci})
      \end{itemize}

    \subsection{Contraction \( \i \)}
      \( \alpha:= a_{1}dx^{1} + a_{2}dx^{2} \in \Omega^{1}(M) \),
      \( \omega:= w_{12}dx^{1}\wedge dx^{2} \in \Omega^{2}(M)\)
      \( \vec{v} := v^{1}\partial_{1} + v^{2}\partial_{2}\in\mathcal{V}(M) \)
      \begin{itemize}
        \item \( \i_{\vec{v}}\alpha = \alpha\left( \vec{v} \right) = a_{1}v^{1} + a_{2}v^{2} \)
        \item \( \i_{\vec{v}}\omega = w_{12}\left( -v^{2}dx^{1} + v^{1}dx^{2} \right) \)
      \end{itemize}

    \subsection{Lie-derivative \( \L \)}
       \( f\in \Omega^{0}(M)\),
       \( \alpha:= a_{1}dx^{1} + a_{2}dx^{2} \in \Omega^{1}(M) \),
       \( \omega:= w_{12}dx^{1}\wedge dx^{2} \in \Omega^{2}(M) \),
       \( \vec{v} := v^{1}\partial_{1} + v^{2}\partial_{2}\in\mathcal{V}(M) \)
       \begin{itemize}
        \item \( \L_{\vec{v}}f = v^{1}\partial_{1}f + v^{2}\partial_{2}f \)
        \item \( \L_{\vec{v}}\alpha = \sum_{i,k=1,2} \left(v^{k}\partial_{k}a_{i}dx^{i} + a_{i}\partial_{k}v^{i}dx^{k}\right) \)
        \item \( \L_{\vec{v}}\omega = \left( \partial_{1}\left( w_{12}v^{1} \right) 
                                        +  \partial_{2}\left( w_{12}v^{2} \right)\right) dx^{1}\wedge dx^{2}\)
        \item \( \L_{\vec{v}}\omega = \left(w_{12}\partial_{\mu}v^{\mu} + v^{\mu}\partial_{\mu}w_{12}\right) dx^{1}\wedge dx^{2} \)
           (\textbf{Ricci})
       \end{itemize}

    \subsection{Levi-Civita-Connection (co-/contravariant derivatives)}
      \begin{itemize}
        \item \( \Gamma_{ij}^{k} = g^{kl}\Gamma_{ijl} = \frac{1}{2}g^{kl}
              \left( \partial_{i}g_{jl} + \partial_{j}g_{il} - \partial_{l}g_{ij} \right) \)
           (\textbf{Christoffel symbols})
        \item \( \nabla_{j}v^{i} = v^{i}_{;j} = v^{i}_{|j} = \partial_{j}v^{i} + v^{k}\Gamma_{jk}^{i} \)
        \item \( \nabla \vec{v} := \left[ \nabla_{j}v^{i} \right]^{i}_{j} \)
        \item \( \left[ \nabla\vecflat{v} \right]_{ji} 
                      = \left[ \left(\nabla\vec{v}\right)g \right]_{ji}
                      = \nabla_{j}v_{i} = v_{i;j} = v_{i|j} = \partial_{j}v_{i} - v_{k}\Gamma_{ij}^{k} 
                      = g_{il}\nabla_{j}v^{l}\)
        \item \( \left[ \nabla^{\sharp}\vecflat{v} \right]_{i}^{j} 
                      = \left[ g^{-1}\left(\nabla\vec{v}\right)g \right]_{i}^{j}
                      = \nabla^{j}v_{i} = v_{i}^{;j} = v_{i}^{|j} 
                      = g^{jk}g_{il}\nabla_{k}v^{l}\)
        \item \( \nabla_{i}f = \left[ \nabla f \right]_{i} = \partial_{i}f \)
        \item \( \nabla_{\vec{v}}f = \L_{\vec{v}}f= \left\langle \vec{v}, \nabla_{\Gamma}f \right\rangle
                  = (\exd f)(\vec{v}) = v^{i}\nabla_{i}f = v^{i}\partial_{i}f \)
      \end{itemize}

    \subsection{Shape-Operator \( S \), etc}
    \begin{itemize}
      \item \textbf{Second fundamental form}:\\
        \( [I\!I]_{ij} = [S^{\flat}]_{ij} = h_{ij} = -\partial_{i}\vec{N}\cdot\partial_{j}\vec{X} 
                      = -\left[ \nabla\vec{N} \right]_{ij}
                      = \vec{n} \cdot \partial_{i}\partial_{j}\vec{X} \)
      \item \textbf{Shape operator (Weingarten map)}:\\
        \( \left[ S \right]^{i}_{j} = g^{ik}h_{kj} = -\left[ \nabla_{\Gamma}\vec{N}\right]^{i} \cdot \partial_{j}\vec{X}
                                    = -\left[\nabla_{\Gamma}\vec{N}\right]^{i}_{j} \)
      \item \textbf{Inverse of second fundamental form}: \\
        \( b^{ij} = \left[ I\!I^{-1}\right]^{ij} = \frac{1}{|g|K}\left[ I\!I^{\text{Adj}}\right]^{ij} \)
      \item \( \left[S(\vec{v})\right]_{i} = -\left[ \nabla_{\vec{v}}\vec{N}\right]_{i} = v^{j}h_{ij} \)
      \item \( S^{T}\alpha = \alpha S =  S(\alpha^{\sharp})   \)
    \end{itemize}

    \subsection{Conclusions}
    \(  \vec{v} := v^{1}\partial_{1} + v^{2}\partial_{2}\in\mathcal{V}(M) \)
    \begin{itemize}
      \item \( \text{Grad}f = \nabla_{\Gamma}f = \nabla^{\sharp}f = \left( \exd f \right)^{\sharp} \)\\
            \( \left[  \text{Grad}f \right]^{i} = \nabla^{i}f =g^{ij}\nabla_{j} f = g^{ij}\partial_{j}f \)
      \item \(
        \begin{aligned}[t]
            \text{Div}\vec{v} &= -\delta\vecflat{v} = *\exd * \vecflat{v} = \nabla_{i}v^{i}
                               = \partial_{i}v^{i} + v^{k}\Gamma_{ik}^{i} 
                               = \partial_{i}v^{i} + v^{k}\partial_{k}\log\sqrt{|g|}\\
                                 &= \sum_{i=1,2} \frac{1}{\sqrt{|g|}}\partial_{i} \sqrt{|g|} v^{i}
                                 = \sum_{i=1,2} \frac{v^{i}}{\sqrt{|g|}}\partial_{i} \sqrt{|g|} + \partial_{i}v^{i}
        \end{aligned}\)\\
      \item
        \( \delta\left( f\alpha \right) = f\delta\alpha - \left\langle \exd f , \alpha \right\rangle \)
      \item
        \( \text{Div} (f\vec{v}) = f\text{Div}\vec{v} + \nabla_{\vec{v}}f = f\nabla_{i}v^{i} + v^{i}\nabla_{i}f  \)
      \item \textbf{Laplace-Beltrami operator}:\\
        \( \Delta_{B}f = -\delta\exd f = *\exd *\exd f = \text{Div}\text{Grad}f = \nabla_{i}\nabla^{i} f
                      = \frac{1}{\sqrt{|g|}}\partial_{j}\left( g^{ij}\sqrt{|g|}\partial_{i}f \right) \)
      \item \textbf{Laplace-de Rham operator}:\\
        \( \Delta_{dR}\alpha = \left( \delta\exd + \exd\delta \right)\alpha =:  -\left( \Delta_{B} + \Delta_{CB} \right)\alpha \)\\
        \( \Delta_{dR}\vec{v} = \left( \Delta_{dR}\vecflat{v} \right)^{\sharp} \)
      \item \textbf{Giaquinta-Hildebrandt operator}:\\
        \( \Delta_{GH}f = \Box f = \text{Div}\left( K II^{-1} \exd f \right)
                                = -\delta\left( KS^{-T}\exd f \right)
                                = \frac{1}{\sqrt{|g|}}\partial_{j}\left( \sqrt{|g|}K b^{ij}\partial_{i}f \right)\)
      \item 
        \( -\delta\left( S^{T}\alpha \right) = -H\Div \alpha^{\sharp} - \Div\left(  K II^{-1} \alpha \right) - \nabla_{\alpha^{\sharp}}H
                            = H\delta\alpha + \delta\left( KS^{-T}\alpha \right) - \left\langle \alpha , \exd H \right\rangle\) 
        \( -\delta\left( S^{T}\exd f \right) = -H\Delta_{B}f - \Delta_{GH}f - \left\langle \exd H , \exd f \right\rangle \)
    \end{itemize}

    \subsection{Moving Surfaces \( M(t) \)}
    \(  \vec{V} := \vec{v} +v_{n}\vec{N} = \partial_{t}\vec{X} \) (surface velocity), \( \vec{X}:M\rightarrow E^{3} \) (parametrization)
    \begin{itemize}
      \item \( \partial_{i}\vec{V}\cdot\partial_{j}\vec{X} = g_{jk}\nabla_{i}v^{k} - v_{n}h_{ij} 
                                                     = \left[\left( \nabla\vec{v} - v_{n}S \right)^{\flat}\right]_{ij}\)
      \item (rate-of-deformation tensor \( \pmb{d} \))\\
        \(\begin{aligned}[t]
            \frac{d}{dt}g &= \left( \nabla\vecflat{v} \right) + \left( \nabla\vecflat{v} \right)^{T} - 2v_{n}I\!I 
                          = \L_{\vec{V}}g = 2 \pmb{d}\\
            \frac{d}{dt}g_{ij} &= g_{ik}\nabla_{j}v^{k} + g_{jk}\nabla_{i}v^{k} - 2v_{n}h_{ij} = 2 d_{ij}
          \end{aligned}\)
      \item
        \(\begin{aligned}[t]
            \left\langle \frac{d}{dt}\vecflat{p} , \alpha \right\rangle
                &= \dot{\vec{p}}\alpha + 2\vec{p}\pmb{d}\alpha^{\sharp}
                = \dot{\vec{p}}\alpha + \vec{p}\left( \left(\nabla\vec{v}\right)^{T} + \left(\nabla^{\sharp}\vecflat{v}\right) 
                       - 2*v_{n}S^{T} \right)\alpha \\
                &= \dot{p}^{i}\alpha_{i} + p^{j}\left( \nabla_{j}v^{i} + \nabla^{i}v_{j} - 2v_{n}h^{i}_{j}\right)\alpha_{i}
          \end{aligned}\)
      \item
        \(\begin{aligned}[t]
             \frac{d}{dt}\alpha^{\sharp} &= \left[ \dot{\alpha} 
                            + \left( 2v_{n}S^{T} 
                            - \left( \nabla\vec{v} \right)^{T} 
                            - \left( \nabla^{\sharp}\vecflat{v} \right) \right)\alpha \right]^{\sharp}         
          \end{aligned}\)
      \item
        \(\begin{aligned}[t]
            \frac{d}{dt}*\omega = *\left[ \dot{\omega}  - \left( \Div\vec{v} + v_{n}H \right)\omega\right]
          \end{aligned}\)
      \item
        \(\begin{aligned}[t]
            \frac{d}{dt}*\vecflat{p} = *\left[ \dot{\vec{p}}  + \left( \Div\vec{v} + v_{n}H \right)\vec{p}\right]^{\flat}
          \end{aligned}\)
      \item
        \(\begin{aligned}[t]
            \frac{d}{dt}*\alpha = *\left[ \dot{\alpha} 
                                          + \left( 2v_{n}S^{T} 
                                                - \left( \nabla\vec{v} \right)^{T} 
                                                - \left( \nabla^{\sharp}\vecflat{v} \right) \right)\alpha
                                          + \left( \Div\vec{v} + v_{n}H \right)\alpha\right]
          \end{aligned}\)
      \item \( 
          \begin{aligned}[t]
          \frac{1}{2} \frac{d}{dt} \left\| \alpha \right\|^{2} 
                &= \left\langle \dot{\alpha} + v_{n}S^{T}\alpha - (\nabla\vec{v})^{T}\alpha , \alpha \right\rangle
                = \dot{\alpha}\alpha^{\sharp} + \alpha \left( v_{n} S - \nabla\vec{v}\right) \alpha^{\sharp} \\
                &= \dot{\alpha}_{i}\alpha^{i} + v_{n}\alpha_{i}h^{i}_{j}\alpha^{j} - \alpha_{i}\left( \nabla_{j}v^{i} \right)\alpha^{j}
          \end{aligned}\)
      \item
        \(\begin{aligned}[t]
            \frac{1}{2} \frac{d}{dt} \left\| \omega \right\|^{2} &= \frac{1}{2} \frac{d}{dt} \left( *\omega \right)^{2}
                     = \left\langle \dot\omega , \omega \right\rangle - \left( \Div\vec{v} + v_{n}H \right) \left\| \omega \right\|^{2} 
          \end{aligned}\)
      \item
        \(\begin{aligned}[t]
            \frac{1}{2} \frac{d}{dt} \left\| \delta\alpha \right\|^{2} 
                  &= \left\langle \delta\left[ \dot{\alpha} 
                                          + \left( 2v_{n}S^{T} 
                                                - \left( \nabla\vec{v} \right)^{T} 
                                                - \left( \nabla^{\sharp}\vecflat{v} \right) \right)\alpha
                                          + \left( \Div\vec{v} + v_{n}H \right)\alpha 
                                            \right] 
                                 , \delta\alpha\right\rangle
                     - \left( \Div\vec{v} + v_{n}H \right) \left\| \delta\alpha \right\|^{2}
          \end{aligned}\)
      \item
        \(\begin{aligned}[t]
            \frac{1}{2} \frac{d}{dt} \left\| \delta\vecflat{p} \right\|^{2} 
                  &= \left\langle \delta\left[ \dot{\vec{p}} 
                                          + \left( \Div\vec{v} + v_{n}H \right)\vec{p} 
                                            \right]^{\flat}
                                 , \delta\vecflat{p}\right\rangle
                     - \left( \Div\vec{v} + v_{n}H \right) \left\| \delta\vecflat{p} \right\|^{2}
          \end{aligned}\)
      \item
        \(\begin{aligned}[t]
            \frac{d}{dt}\int_{M(t)} f \mu = \int_{M(t)} \dot{f} + f\left( \Div\vec{v} + v_{n}H \right) \mu
          \end{aligned}\)
      \item
        \(\begin{aligned}[t]
              \frac{d}{dt}\int_{M(t)} \frac{1}{2} \left\| \alpha \right\|^{2} \mu
                  = \int_{M(t)} \left\langle \dot\alpha, \alpha \right\rangle
                                + v_{n}\left\langle S^{T}\alpha + \frac{1}{2}H\alpha, \alpha \right\rangle
                                + \left\langle \frac{1}{2}\left(\Div\vec{v}\right)\alpha - (\nabla\vec{v})^{T}\alpha , \alpha \right\rangle
                    \mu
          \end{aligned}\)
      \item
        \(\begin{aligned}[t]
            \frac{d}{dt}\int_{M(t)} \frac{1}{2} \left\| \omega \right\|^{2} \mu
                &= \int_{M(t)} \left\langle \dot\omega , \omega \right\rangle 
                            - \frac{1}{2}\left( \Div\vec{v} + v_{n}H \right) \left\| \omega \right\|^{2} \mu \\
          \end{aligned}\)
      \item
        \(\begin{aligned}[t]
            \frac{d}{dt}\int_{M(t)} \frac{1}{2} \left\| \exd\vecflat{p} \right\|^{2} \mu
                &= \int_{M(t)} \left\langle\frac{d}{dt}\vecflat{p}, \delta\exd\vecflat{p}\right\rangle
                            - \frac{1}{2}\left( \Div\vec{v} + v_{n}H \right) \left\| \exd\vecflat{p} \right\|^{2} \mu \\
                &= \int_{M(t)} \dot{\vec{p}}\delta\exd\vecflat{p} 
                      + \vec{p}\left( \left(\nabla\vec{v}\right)^{T} + \left(\nabla^{\sharp}\vecflat{v}\right) 
                       - 2v_{n}S^{T} \right)\delta\exd\vecflat{p}\\
                &\hspace{1cm}            - \frac{1}{2}\left( \Div\vec{v} + v_{n}H \right) \left\| \exd\vecflat{p} \right\|^{2} \mu \\
          \end{aligned}\)
      \item
        \(\begin{aligned}[t]
            \frac{d}{dt}\int_{M(t)} \frac{1}{2} \left\| \delta\vecflat{p} \right\|^{2} \mu
                &= \int_{M(t)}\left\langle\frac{d}{dt}\vecflat{p}, \exd\delta\vecflat{p}\right\rangle
                  + \left\langle \left( 2v_{n}S^{T} - \left(\nabla\vec{v}\right)^{T} - \left(\nabla^{\sharp}\vecflat{v}\right)\right)\vecflat{p}
                                  , \exd\delta\vecflat{p} \right\rangle
                  \\&\hspace{1cm}  
                  + \left\langle \left( \Div\vec{v} + v_{n}H \right)\vecflat{p} , \exd\delta\vecflat{p} \right\rangle
                  - \frac{1}{2}\left( \Div\vec{v} + v_{n}H \right)\left\| \delta\vecflat{p} \right\|^{2} \mu \\
                &=  \int_{M(t)} \dot{\vec{p}}\exd\delta\vecflat{p}
                      + \left( \Div\vec{v} + v_{n}H \right)\vec{p}\exd\delta\vecflat{p}
                      - \frac{1}{2}\left( \Div\vec{v} + v_{n}H \right)\left\| \delta\vecflat{p} \right\|^{2} \mu 
          \end{aligned}\)
      \item
        \(\begin{aligned}[t]
            \frac{d}{dt}\int_{M(t)} \frac{1}{2}\left( \left\| \exd\vecflat{p} \right\|^{2} + \left\| \delta\vecflat{p} \right\|^{2} \right)\mu
                &=  \frac{d}{dt}\int_{M(t)} \frac{1}{2}\left( \left\| \Rot\vec{p} \right\|^{2} 
                                                            + \left\| \Div\vec{p} \right\|^{2} \right)\mu \\
                &= \int_{M(t)} \left\langle\frac{d}{dt}\vecflat{p}, \Delta_{dR}\vecflat{p}\right\rangle 
                    - \frac{\Div\vec{v} + v_{n}H}{2}\left( \left\| \exd\vecflat{p} \right\|^{2} + \left\| \delta\vecflat{p} \right\|^{2}  \right)
                \\&\hspace{1cm}
                  + \left\langle \left( \Div\vec{v} + v_{n}H \right)\vecflat{p} , \exd\delta\vecflat{p} \right\rangle
                \\&\hspace{1cm}
                  - \left\langle \left(\left(\nabla\vec{v}\right)^{T} + \left(\nabla^{\sharp}\vecflat{v}\right) - 2v_{n}S^{T}\right)\vecflat{p}
                                  , \exd\delta\vecflat{p} \right\rangle \mu\\
                &= \int_{M(t)} \left\langle \dot{\vec{p}}, \Delta_{dR}\vec{p}\right\rangle 
                    - \frac{\Div\vec{v} + v_{n}H}{2}\left( \left\| \Rot\vec{p} \right\|^{2} 
                                                            + \left\| \Div\vec{p} \right\|^{2}  \right)
                \\&\hspace{1cm}
                  +  \left( \Div\vec{v} + v_{n}H \right)\vec{p} \exd\delta\vecflat{p}
                \\&\hspace{1cm}
                  + \vec{p}\left(\left(\nabla\vec{v}\right)^{T} + \left(\nabla^{\sharp}\vecflat{v}\right) - 2v_{n}S^{T}\right)\delta\exd\vecflat{p} \mu\\
          \end{aligned}\)
      \item
        \(\begin{aligned}[t]
            \int_{M(t)} \left\langle \left( \Div\vec{v} + v_{n}H \right)\vecflat{p} , \exd\delta\vecflat{p} \right\rangle
                  - \frac{1}{2}\left( \Div\vec{v} + v_{n}H \right)\left\| \delta\vecflat{p} \right\|^{2} \mu &\\
              &\hspace{-7cm} = \int_{M(t)} \L_{\vec{p}}\left\langle \vecflat{p}, \exd\delta\vecflat{v} + \exd\left( v_{v}H \right) \right\rangle
                                    + \frac{1}{2}\left( \Div\vec{v} + v_{n}H \right)\left\| \delta\vecflat{p} \right\|^{2}\mu
          \end{aligned}\)

    \end{itemize}
        
  
\end{document}
